theories/Vector.v
@@ -7,15 +7,32 @@ Import Coq.NArith.BinNat.
 
 Record vector {A n} := {
   vector_list : list A;
-  vector_wf : N.of_nat (length vector_list) = n;
+  vector_wf : length_bin vector_list = n;
 }.
 
 Arguments vector : clear implicits.
+
+Notation bitvec := (vector bool).
+
+Notation "[| |]" := {| vector_list := []; vector_wf := eq_refl |} (format "[| |]").
+Notation "[| x |]" := {| vector_list := [x]; vector_wf := eq_refl |}.
+Notation "[| x ; y ; .. ; z |]" := {| vector_list := cons x (cons y .. [z] ..); vector_wf := eq_refl |}.
 
 Register vector as vcpu.vector.type.
 Register Build_vector as vcpu.vector.constructor.
 Register vector_list as vcpu.vector.list.
 Register vector_wf as vcpu.vector.wf.
+
+#[program] Definition vector_head {A n} (v : vector A (N.succ n)) : A :=
+  match vector_list v with
+  | x :: _ => x
+  | [] => _
+  end.
+Next Obligation.
+  intros A n v. specialize (vector_wf v) as H. destruct (vector_list v).
+  - simpl in H. apply N.neq_0_succ in H. destruct H.
+  - simpl. auto.
+Qed.
 
 #[program] Definition vector_tail {A n} (v : vector A (N.succ n)) : vector A n := {|
   vector_list := List.tl (vector_list v);
@@ -23,10 +40,22 @@ Register vector_wf as vcpu.vector.wf.
 Next Obligation.
   intros A n v. specialize (vector_wf v) as H. destruct (vector_list v).
   - simpl in H. apply N.neq_0_succ in H. destruct H.
-  - simpl. simpl in H. lia.
+  - simpl. rewrite length_bin_cons in H. apply N.succ_inj in H. auto.
 Qed.
 
-Notation bitvec := (vector bool).
+Definition vector_dest {A n} (v : vector A (N.succ n)) : A * vector A n :=
+  (vector_head v, vector_tail v).
+
+Register vector_dest as vcpu.vector.dest.
+
+#[program] Definition vector_app {A n1 n2} (v1 : vector A n1) (v2 : vector A n2) : vector A (n1 + n2) := {|
+  vector_list := vector_list v1 ++ vector_list v2;
+|}.
+Next Obligation.
+  intros A n1 n2 v1 v2. rewrite length_bin_app. rewrite ? vector_wf. auto.
+Qed.
+
+Register vector_app as vcpu.vector.app.
 
 Unset Program Cases.
 
@@ -34,10 +63,8 @@ Unset Program Cases.
   vector_list := List.map (fun '(b1, b2) => f b1 b2) (List.combine (vector_list bv1) (vector_list bv2));
 |}.
 Next Obligation.
-  intros f n bv1 bv2. rewrite List.map_length. rewrite List.combine_length.
-  rewrite <- (Nnat.Nat2N.id (length (vector_list bv1))).
-  rewrite <- (Nnat.Nat2N.id (length (vector_list bv2))).
-  rewrite ? vector_wf. rewrite PeanoNat.Nat.min_id. lia.
+  intros f n bv1 bv2. rewrite length_bin_list_map. rewrite length_bin_list_combine.
+  rewrite ? vector_wf. apply N.min_id.
 Qed.
 
 Set Program Cases.
